ambient_capabilities_coq_model/assert_theory.v
@@ -17,15 +17,13 @@ Module AssertTheory.
   Import OperationalSemantics.
   Import Assert.
 
-  Definition entails (M : module)(A1 A2 : asrt) : Prop := forall σ, sat M σ (A1 ⟶ A2).
+  Parameter entails : module -> asrt -> asrt -> Prop.
+
+  (*Definition entails (M : module)(A1 A2 : asrt) : Prop := forall σ, sat M σ (A1 ⟶ A2).*)
 
   Notation "M ⊢ A1 ⊆ A2" := (entails M A1 A2)(at level 40).
 
-  Lemma entails_strengthening :
-    forall M σ A1 A2, sat M σ A1 ->
-                 sat M σ (A1 ⟶ A2) ->
-                 sat M σ A2.
-  Proof.
-  Admitted.
+  Parameter entails_sound :
+    forall M A1 A2, entails M A1 A2 <-> (forall σ, sat M σ A1 -> sat M σ A2).
 
 End AssertTheory.
