ambient_capabilities_coq_model/spec.v
@@ -46,7 +46,10 @@ Module SpecSatisfaction.
   | spec_method : forall M C meth A1 A2 A3 CDef m,
       snd M C = Some CDef ->
       c_meths CDef meth = Some m ->
-      M ⊢ ⦃ a_typs ((result, rtrn m)::(this, t_cls C) :: (params m)) ∧ A1 ⦄
+      M ⊢ ⦃ a_typs ((result, rtrn m)::
+                      (this, t_cls C) ::
+                      (params m)) ∧
+              A1 ⦄
         (body m)
         ⦃ A2 ∧ (adapt A2 (result :: nil)) ⦄ ||
         ⦃ A3 ⦄ ->
@@ -56,8 +59,11 @@ Module SpecSatisfaction.
       (forall C CDef m meth,
           snd M C = Some CDef ->
           c_meths CDef meth = Some m ->
+          vis m = public ->
           M ⊢
-            ⦃ a_typs ((result, rtrn m)::(this, t_cls C) :: (params m)) ∧
+            ⦃ a_typs ((result, rtrn m)::
+                      (this, t_cls C) ::
+                      (params m)) ∧
                 (a_typs (map (fun xC => (fst xC, t_cls (snd xC))) xCs)) ∧ A ⦄
             (body m)
             ⦃ A ∧ (adapt A (result :: nil)) ⦄ || ⦃ A ⦄) ->
